more

thys/Common_Rec_Corec/Comodels.thy
@@ -9,10 +9,10 @@ definition dtorPermC :: "('E' \<Rightarrow> bool) \<Rightarrow>
 ('E' \<Rightarrow> 'a E + ('a::var,'a,'E','E')G set) \<Rightarrow> 
 (('a \<Rightarrow> 'a) \<Rightarrow> 'E' \<Rightarrow> 'E') \<Rightarrow> bool" 
 where "dtorPermC valid dtor perm \<equiv> 
-\<forall>\<sigma> e. valid e \<and> small \<sigma> \<and> bij \<sigma> \<longrightarrow> 
-  (\<forall> U. dtor e = Inr U \<longrightarrow> (\<exists>U'. dtor (perm \<sigma> e) = Inr U' \<and> U' \<subseteq> Gren \<sigma> \<sigma> ` (Gmap (perm \<sigma>) (perm \<sigma>) ` U)))
+\<forall>\<sigma> e. valid e \<and> small \<sigma> \<and> bij \<sigma> \<longrightarrow>
+  (\<forall>e1. dtor e = Inl e1 \<longrightarrow> dtor (perm \<sigma> e) = Inl (Eperm \<sigma> e1))
   \<and> 
-  (\<forall>e1. dtor e = Inl e1 \<longrightarrow> dtor (perm \<sigma> e) = Inl (Eperm \<sigma> e1))"
+  (\<forall> U. dtor e = Inr U \<longrightarrow> (\<exists>U'. dtor (perm \<sigma> e) = Inr U' \<and> U' \<subseteq> Gren \<sigma> \<sigma> ` (Gmap (perm \<sigma>) (perm \<sigma>) ` U)))"
 
 definition dtorVrsGrenC :: "('E' \<Rightarrow> bool) \<Rightarrow> 
 ('E' \<Rightarrow> 'a E + ('a::var,'a,'E','E')G set) \<Rightarrow> 
